Unfold definitions to highlight a bug.

examples/Stocks.v
@@ -84,12 +84,21 @@ Definition StocksSpec : ADT StocksSig :=
             Return (N.mul transaction!PRICE transaction!VOLUME))
 }.
 
+Definition StocksHeading := GetHeading StocksSchema STOCKS.
+Definition TransactionsHeading := GetHeading StocksSchema TRANSACTIONS.
+
+(* Using those breaks refine_foreign_key_check_into_query *)
+Definition STOCK_STOCKCODE        := StocksHeading/STOCK_CODE.
+Definition STOCK_TYPE             := StocksHeading/TYPE.
+Definition TRANSACTIONS_DATE      := TransactionsHeading/DATE.
+Definition TRANSACTIONS_STOCKCODE := TransactionsHeading/STOCK_CODE.
+
 Definition StocksStorage : @BagPlusBagProof (StocksSchema#STOCKS).
-  makeIndex StocksSchema STOCKS [ TYPE; STOCK_CODE ].
+  mkIndex StocksHeading [StocksHeading/TYPE; StocksHeading/STOCK_CODE].
 Defined.
 
 Definition TransactionsStorage : @BagPlusBagProof (StocksSchema#TRANSACTIONS).
-  makeIndex StocksSchema TRANSACTIONS [ DATE; STOCK_CODE ].
+  mkIndex TransactionsHeading [TransactionsHeading/DATE; TransactionsHeading/STOCK_CODE].
 Defined.
 
 Definition TStocksBag := BagType StocksStorage.
@@ -103,7 +112,64 @@ Definition Stocks_AbsR
 Definition StocksDB :
   Sharpened StocksSpec.
 Proof.
+  match goal with
+    | [ |- Sharpened ?spec ] =>
+      unfolder spec ltac:(fun spec' => change spec with spec')
+  end; start_honing_QueryStructure; hone_representation Stocks_AbsR.
+
+(*  plan Stocks_AbsR. *)
+ 
+  hone method "AddTransaction".
+  startMethod Stocks_AbsR. 
+  pruneDuplicates. 
+  pickIndex.
+  fundepToQuery.
+  concretize.
+  asPerm (StocksStorage, TransactionsStorage).
+  commit.
+
+  (* This is the body of foreignToQuery *) 
+  match goal with
+    | [ |- context[Pick (fun b' => decides b' (exists tup2 : @IndexedTuple ?H, _ /\ ?r ``?s = _ ))] ] =>
+      match goal with
+        | [ |- appcontext[@benumerate _ (@Tuple ?H')] ] =>
+          equate H H'; let T' := constr:(@Tuple H') in
+                       let temp := fresh in
+                       pose (refine_foreign_key_check_into_query (fun t : T' => r!s = t!s)) as temp;
+                         rewrite temp by eauto with typeclass_instances;
+                         simplify with monad laws; cbv beta; simpl; clear temp
+      end
+  end.
+
+  Focus 2.
+  (* Strange thing: there are two levels of absMethod here *)
+  hone method "LargestTransaction". 
+  idtac.
+  idtac.
+  unfold Stocks_AbsR in *; split_and. simplify with monad laws.
+  startMethod Stocks_AbsR. concretize. asPerm (StocksStorage, TransactionsStorage.
+  commit; choose_db AbsR; finish honing.
+  
+  match goal with
+    | [ |- Sharpened ?spec ] =>
+      unfolder spec ltac:(fun spec' => change spec with spec')
+  end; start_honing_QueryStructure. hone_representation Stocks_AbsR.
+
+  hone method "AddStock".
+  mutator.
+  startMethod Stocks_AbsR; repeat progress (try setoid_rewrite refine_trivial_if_then_else; 
+                   try setoid_rewrite key_symmetry;
+                   try setoid_rewrite refine_tupleAgree_refl_True; 
+                   try simplify with monad laws); pickIndex;
+  repeat ((foreignToQuery || fundepToQuery);
+          concretize; asPerm storages; commit);
+  Split Constraint Checks; checksSucceeded || checksFailed.
+  pickIndex.
+  mutator.
+  honeOne.
+
   plan Stocks_AbsR.
+  
   Print Ltac plan.
 
   (*unfold cast, eq_rect_r, eq_rect, eq_sym.*)
